LogicalHeaps WIP

bin/rust/rocq/LogicalHeaps.v
@@ -21,6 +21,8 @@ Parameter lh_sing: PrimChunk → LogHeap.
 
 Declare Scope logheap_scope.
 
+Notation "∅" := lh_empty (format "∅") : logheap_scope.
+
 Infix "⋅" := lh_comp (at level 50, left associativity) : logheap_scope.
 
 Open Scope logheap_scope.
@@ -33,85 +35,384 @@ Infix "≼" := lh_le (at level 70) : logheap_scope.
 Notation "{[+ x +]}" := (lh_sing x)
   (at level 1, format "{[+ x +]}") : logheap_scope.
 
-Require KnasterTarski.
-
-Module LogHeapPredTarskiParams.
-  Definition X: Type := string * list Value * LogHeap.
-End LogHeapPredTarskiParams.
-
-Module Tarski_ := KnasterTarski.Predicates LogHeapPredTarskiParams.
-Module Tarski := Tarski_.T.
+Axiom lh_left_id: forall H, ∅ ⋅ H = H.
+Axiom lh_right_id: forall H, H ⋅ ∅  = H.
+Axiom lh_assoc: forall H1 H2 H3, H1 ⋅ (H2 ⋅ H3) = (H1 ⋅ H2) ⋅ H3.
+Axiom lh_comm: forall H1 H2, H1 ⋅ H2 = H2 ⋅ H1.
 
 Section preds.
 
 Variable preds: list (string * PredDef).
 
-Section pred_interp.
+Inductive pat_matches: forall (env: Env)(pat: Pat)(v: Value)(env': Env), Prop :=
+| LitPat_matches env e v:
+  eval env e = v →
+  pat_matches env (LitPat e) v env
+| VarPat_matches env x v:
+  pat_matches env (VarPat x) v ((x, LSValue v)::env)
+.
 
-Variable pred_interp: string * list Value * LogHeap -> Prop.
+Inductive pats_match: forall (env: Env)(pats: list Pat)(vs: list Value)(env': Env), Prop :=
+| empty_pats_match env:
+  pats_match env [] [] env
+| nonempty_pats_match env pat pats v vs env' env'':
+  pat_matches env pat v env' →
+  pats_match env' pats vs env'' →
+  pats_match env (pat::pats) (v::vs) env''
+.
 
-Fixpoint lh_consume(H: LogHeap)(env: Env)(a: Asn)(Q: LogHeap → Env → Prop): Prop :=
-  match a with
-    BoolAsn e => eval env e = VBool true ∧ Q H env
-  | PointsToAsn ty ptr rhs =>
-    ∃ v H',
-    H = {[+ PointsTo ty (eval env ptr) v +]} ⋅ H' ∧
-    match_pat env rhs v @@ fun env =>
-    Q H' env
-  | PredAsn pred_name pats =>
-    ∃ vs Hp H',
-    H = Hp ⋅ H' ∧
-    pred_interp (pred_name, vs, Hp) ∧
-    match_pats [] env pats vs @@ fun env =>
-    Q H' env
-  | SepAsn a1 a2 =>
-    lh_consume H env a1 @@ fun H env =>
-    lh_consume H env a2 Q
-  | IfAsn cond a1 a2 =>
-    (eval env cond = VBool true → lh_consume H env a1 Q) ∧
-    (eval env cond ≠ VBool true → lh_consume H env a2 Q)
-  end.
+Inductive asn_holds: forall (H: LogHeap)(env: Env)(a: Asn)(env': Env), Prop :=
+| BoolAsn_holds H env e:
+  eval env e = VBool true →
+  H = ∅ →
+  asn_holds H env (BoolAsn e) env
+| PointsToAsn_holds H env ty ptr pat v env':
+  H = {[+ PointsTo_ ty (eval env ptr) (VSome v) +]} →
+  pat_matches env pat v env' →
+  asn_holds H env (PointsToAsn ty ptr pat) env'
+| PredAsn_holds H env pred_name pats vs env' params body env'' env''':
+  assoc pred_name preds = Some {| params := params; body := body |} →
+  combine_ params vs = (env'', ([], [])) →
+  asn_holds H (map (fun '((x, ty), v) => (x, LSValue v)) env'') body env''' →
+  pats_match env pats vs env' →
+  asn_holds H env (PredAsn pred_name pats) env'
+| SepAsn_holds H1 H2 env a1 env' a2 env'':
+  asn_holds H1 env a1 env' →
+  asn_holds H2 env' a2 env'' →
+  asn_holds (H1 ⋅ H2) env (SepAsn a1 a2) env''
+| IfAsn_holds_true H env cond a1 a2 env':
+  eval env cond = VBool true →
+  asn_holds H env a1 env' →
+  asn_holds H env (IfAsn cond a1 a2) env'
+| IfAsn_holds_false H env cond a1 a2 env':
+  eval env cond ≠ VBool true →
+  asn_holds H env a2 env' →
+  asn_holds H env (IfAsn cond a1 a2) env'
+.
 
-Definition asn_holds(H: LogHeap)(env: Env)(a: Asn): Prop :=
-  lh_consume H env a @@ fun _ _ => True.
-
-Definition pred_holds_ '(pred_name, args, H): Prop :=
-  match assoc pred_name preds with
-    None => False
-  | Some {| params := params; body := body |} =>
-    match combine_ params args with
-      (bindings, ([], [])) =>
-      let env := map (fun '((x, ty), v) => (x, LSValue v)) bindings in
-      asn_holds H env body
-    | _ => False
+Definition chunk_holds(H: LogHeap)(chunk: Chunk): Prop :=
+  match chunk with
+    Prim chunk => H = {[+ chunk +]}
+  | PointsTo ty ptr v => H = {[+ PointsTo_ ty ptr (VSome v) +]}
+  | User pred_name vs =>
+    match assoc pred_name preds with
+      None => False
+    | Some {| params := params; body := body |} =>
+      match combine_ params vs with
+        (env, ([], [])) =>
+        ∃ env', asn_holds H (map (fun '((x, ty), v) => (x, LSValue v)) env) body env'
+      | _ => False
+      end
     end
   end.
 
-End pred_interp.
+Fixpoint heap_holds(H: LogHeap)(h: Heap): Prop :=
+  match h with
+    [] => H = ∅
+  | chunk::chunks =>
+    ∃ H1 H2,
+    H = H1 ⋅ H2 ∧ chunk_holds H1 chunk ∧ heap_holds H2 chunks
+  end.
 
-Lemma pred_holds_mono
-    (pred_interp1: string * list Value * LogHeap -> Prop)
-    (pred_interp2: string * list Value * LogHeap -> Prop):
-  (forall chunk, pred_interp1 chunk -> pred_interp2 chunk) ->
-  (forall chunk, pred_holds_ pred_interp1 chunk -> pred_holds_ pred_interp2 chunk).
+Lemma heap_holds_append(H1 H2: LogHeap)(h1 h2: Heap):
+  heap_holds H1 h1 →
+  heap_holds H2 h2 →
+  heap_holds (H1 ⋅ H2) (h1 ++ h2).
 Proof.
+  revert H1 H2 h2.
+  induction h1; intros H1 H2 h2 Hh1 Hh2; simpl in *; subst.
+  - (* nil *)
+    rewrite lh_left_id.
+    assumption.
+  - (* cons *)
+    destruct Hh1 as (Hchunk & Hh1 & HH1 & HHchunk & HHh1).
+    exists Hchunk.
+    exists (Hh1 ⋅ H2).
+    split. {
+      rewrite HH1.
+      rewrite lh_assoc.
+      reflexivity.
+    }
+    split. assumption.
+    apply IHh1; assumption.
+Qed.
+
+Lemma nth__iter_sound(H_done H_todo: LogHeap)(k: nat)(h_done h_todo: Heap)(chunk: Chunk)(h: Heap):
+  heap_holds H_done h_done →
+  heap_holds H_todo h_todo →
+  nth__iter k h_done h_todo = Some (chunk, h) →
+  ∃ Hchunk Hh,
+  H_done ⋅ H_todo = Hchunk ⋅ Hh ∧
+  chunk_holds Hchunk chunk ∧
+  heap_holds Hh h.
+Proof.
+  revert H_done H_todo h_done h_todo chunk h.
+  induction k; intros H_done H_todo h_done h_todo chunk h Hh_done Hh_todo Hnth__iter.
+  - (* O *)
+    destruct h_todo as [|chunk' h']; try discriminate.
+    simpl in Hnth__iter.
+    injection Hnth__iter; intros; subst.
+    inversion Hh_todo.
+    rename x into Hchunk.
+    rename H into HH_todo.
+    destruct HH_todo as [Hh' [HH_todo [HHchunk HHh']]].
+    exists Hchunk.
+    exists (H_done ⋅ Hh').
+    split. {
+      rewrite lh_assoc.
+      rewrite lh_comm with (H1:=Hchunk).
+      rewrite <- lh_assoc.
+      congruence.
+    }
+    split. assumption.
+    apply heap_holds_append; assumption.
+  - (* S k *)
+    destruct h_todo as [|chunk' h']; try discriminate.
+    simpl in Hnth__iter.
+    inversion Hh_todo.
+    rename x into Hchunk'.
+    rename H into HH_todo.
+    destruct HH_todo as [H' [HH_todo [HHchunk' Hh']]].
+    destruct (IHk (Hchunk' ⋅ H_done) H' (chunk'::h_done) h' chunk h) as [Hchunk [Hh [Hchunk1 [Hchunk2 HHh]]]].
+    + simpl.
+      exists Hchunk'.
+      exists H_done.
+      tauto.
+    + assumption.
+    + assumption.
+    + exists Hchunk.
+      exists Hh.
+      split. {
+        rewrite HH_todo.
+        rewrite <- Hchunk1.
+        rewrite lh_comm with (H2:=H_done).
+        apply lh_assoc.
+      }
+      tauto.
+Qed.
+
+Lemma nth__sound(H: LogHeap)(h: Heap)(k: nat)(chunk: Chunk)(h': Heap):
+  heap_holds H h →
+  nth_ k h = Some (chunk, h') →
+  ∃ Hchunk Hh',
+  H = Hchunk ⋅ Hh' ∧
+  chunk_holds Hchunk chunk ∧
+  heap_holds Hh' h'.
+Proof.
+  intros.
+  unfold nth_ in H1.
+  apply nth__iter_sound with (H_done:=∅) (2:=H0) in H1. 2:{
+    simpl.
+    reflexivity.
+  }
+  destruct H1 as (Hchunk & Hh & HH & HHchunk & Hh').
+  exists Hchunk.
+  exists Hh.
+  rewrite lh_left_id in HH.
+  tauto.
+Qed.
+
+Lemma consume_chunk_sound(H: LogHeap)(trace: Trace)(h: Heap)(tree: SymexTree)(Q: Heap → SymexTree → Chunk → Prop):
+  heap_holds H h →
+  consume_chunk trace h tree Q →
+  ∃ Hchunk H' h' tree' chunk,
+  H = Hchunk ⋅ H' ∧
+  chunk_holds Hchunk chunk ∧
+  heap_holds H' h' ∧
+  Q h' tree' chunk.
+Proof.
+  revert H trace h Q.
+  induction tree; intros; try tauto.
+  destruct data; try tauto.
+  - (* ConsumeChunk *)
+    simpl in H1.
+    case_eq (nth_ chunk_index h); intros; rewrite H2 in H1; try tauto.
+    destruct p as [chunk h'].
+    apply nth__sound with (1:=H0) in H2.
+    destruct H2 as (Hchunk & Hh' & HH & HHchunk & H').
+    exists Hchunk.
+    exists Hh'.
+    exists h'.
+    exists tree.
+    exists chunk.
+    tauto.
+  - (* AutoOpen *)
+    simpl in H1.
+    case_eq (nth_ chunk_index h); intros; rewrite H2 in H1; try tauto.
+    destruct p as [chunk h'].
+    destruct chunk; try tauto.
+    apply nth__sound with (1:=H0) in H2.
+    destruct H2 as (Hchunk & Hh' & HH & HHchunk & H').
+    simpl in HHchunk.
+    apply IHtree with (H:=H) (2:=H1).
+    simpl.
+    exists Hchunk.
+    exists Hh'.
+    split. assumption.
+    split. {
+      rewrite HHchunk.
+      reflexivity.
+    }
+    assumption.
+Qed.
+
+Lemma consume_points_to_sound H trace h tree ty ptr Q:
+  heap_holds H h →
+  consume_points_to trace h tree ty ptr Q →
+  ∃ H' h' tree' v,
+  H = {[+ PointsTo_ ty ptr (VSome v) +]} ⋅ H' ∧
+  heap_holds H' h' ∧
+  Q h' tree' v.
+Proof.
+  intros.
+  unfold consume_points_to in H1.
+  apply consume_chunk_sound with (1:=H0) in H1.
+  destruct H1 as (Hchunk & H' & h' & tree' & chunk & ? & ? & ?).
+  destruct chunk; try tauto.
+  destruct H3 as (? & ? & ? & ?).
+  subst.
+  simpl in H2.
+  exists H'.
+  exists h'.
+  exists tree'.
+  exists rhs.
+  split. {
+    rewrite H2.
+    reflexivity.
+  }
+  tauto.
+Qed.
+
+Lemma match_pat_sound env pat v Q:
+  match_pat env pat v Q →
+  ∃ env',
+  pat_matches env pat v env' ∧
+  Q env'.
+Proof.
+  destruct pat; simpl; intros.
+  - (* LitPat *)
+    destruct H.
+    subst.
+    exists env.
+    split. {
+      constructor.
+      reflexivity.
+    }
+    assumption.
+  - (* VarPat *)
+    exists ((x, LSValue v)::env).
+    split. {
+      constructor.
+    }
+    assumption.
+Qed.
+
+Lemma match_pats_sound trace env pats vs Q:
+  match_pats trace env pats vs Q →
+  ∃ env',
+  pats_match env pats vs env' ∧
+  Q env'.
+Proof.
+  revert trace env vs Q.
+  induction pats.
+  - (* nil *)
+    intros trace env vs Q ?.
+    destruct vs; try tauto.
+    exists env.
+    split. constructor.
+    assumption.
+  - (* cons *)
+    intros trace env vs Q ?.
+    destruct vs as [|v vs]; try tauto.
+    simpl in H.
+    apply match_pat_sound in H.
+    destruct H as [env' [? ?]].
+    apply IHpats in H0.
+    destruct H0 as [env'' [? ?]].
+    exists env''.
+    split. {
+      apply nonempty_pats_match with (env':=env'); assumption.
+    }
+    assumption.
+Qed.
+
+Lemma consume_sound(H: LogHeap)(trace: Trace)(h: Heap)(env: Env)(tree: SymexTree)(a: Asn)(Q: Heap → Env → SymexTree → Prop):
+  heap_holds H h →
+  consume trace h env tree a Q →
+  ∃ h' env' tree' H1 H2,
+  H = H1 ⋅ H2 ∧ asn_holds H1 env a env' ∧
+  heap_holds H2 h' ∧
+  Q h' env' tree'.
+Proof.
+  revert H trace h env tree Q.
+  induction a; intros H trace h env tree Q Hh Hconsume; simpl in Hconsume.
+  - (* BoolAsn *)
+    exists h.
+    exists env.
+    exists tree.
+    exists ∅.
+    exists H.
+    split. {
+      rewrite lh_left_id.
+      reflexivity.
+    }
+    assert (HeQ: eval env e = VBool true ∧ Q h env tree). {
+      destruct e; simpl in Hconsume; try tauto.
+      destruct b; tauto.
+    }
+    destruct HeQ as [He HQ].
+    split. {
+      constructor.
+      - assumption.
+      - reflexivity.
+    }
+    tauto.
+  - (* PointsToAsn *)
+    apply consume_points_to_sound with (1:=Hh) in Hconsume.
+    destruct Hconsume as (H' & h' & tree' & v & HH & HH' & ?).
+    apply match_pat_sound in H0.
+    destruct H0 as [env' [? ?]].
+    exists h'.
+    exists env'.
+    exists tree'.
+    exists {[+ PointsTo_ ty (eval env ptr) (VSome v) +]}.
+    exists H'.
+    split. assumption.
+    split. {
+      apply PointsToAsn_holds with (v:=v); tauto.
+    }
+    tauto.
+  - (* PredAsn *)
+    apply consume_chunk_sound with (1:=Hh) in Hconsume.
+    destruct Hconsume as (Hchunk & H' & h' & tree' & chunk & HH & HHchunk & HH' & ?).
+    destruct chunk; try tauto.
+    apply match_pats_sound in H0.
+    destruct H0 as [env' [? ?]].
+    exists h'.
+    exists env'.
+    exists tree'.
+    exists Hchunk.
+    exists H'.
+    split. assumption.
+    split. {
+      simpl in HHchunk.
+      case_eq (assoc pred_name0 preds); intros; rewrite H2 in HHchunk; try tauto.
+      destruct p as [params body].
+      case_eq (combine_ params args0); intros; rewrite H3 in HHchunk.
+      rename l into env''.
+      destruct p as [params' args'].
+      destruct params'; try tauto.
+      destruct args'; try tauto.
+      
+      apply PredAsn_holds with (vs:=args0) (params:=params) (body:=body).
+    
 Admitted.
 
-Definition pred_interp: string * list Value * LogHeap -> Prop := Tarski.fp pred_holds_.
-
-Definition pred_holds := pred_holds_ pred_interp.
-
-Lemma pred_fold(pred_name: string)(args: list Value)(H: LogHeap):
-  pred_holds (pred_name, args, H) -> pred_interp (pred_name, args, H).
-Proof.
-  apply (Tarski.tarski_left _ pred_holds_mono).
-Qed.
-
-Lemma pred_unfold(pred_name: string)(args: list Value)(H: LogHeap):
-  pred_interp (pred_name, args, H) -> pred_holds (pred_name, args, H).
-Proof.
-  apply (Tarski.tarski_right _ pred_holds_mono).
-Qed.
+Lemma produce_sound(H0: LogHeap)(H: LogHeap)(trace: Trace)(h: Heap)(env: Env)(tree: SymexTree)(a: Asn)(env': Env)(Q: Heap → Env → SymexTree → Prop):
+  heap_holds H0 h →
+  asn_holds H env a env' →
+  produce trace h env tree a Q →
+  ∃ h' tree',
+  Q h' env' tree' ∧ heap_holds (H0 ⋅ H) h'.
 
 End preds.
-
